Sketch of simulation proof.
In the PDF, this is the brand new lemma 3.8. It says that any two terms
that have the same skeleton are in bisimulation. Together with Lemma 3.9
and the adequacy of the logical relation, this gives a way to prove that
a syntactic term is safe.

theories/AAsynToSem.v
@@ -1,6 +1,8 @@
 (** Define translation from syntactic terms/values to semantic ones, following Sec. 3.2 of the PDF. *)
 From Dot Require Import tactics synFuncs operational.
 From iris.proofmode Require Import tactics.
+From iris.program_logic Require Import ectx_lifting.
+Import operational.lang.
 
 Section Sec.
   Context `{HdotG: dotG Σ}.
@@ -255,81 +257,81 @@ Section Sec.
   Qed.
 
 
-  Fixpoint same_skel_tm (σ: vls) (t1 t2: tm): Prop :=
+  Fixpoint same_skel_tm (t1 t2: tm): Prop :=
     match (t1, t2) with
-    | (tv v1, tv v2) => same_skel_vl σ v1 v2
+    | (tv v1, tv v2) => same_skel_vl v1 v2
     | (tapp t11 t12, tapp t21 t22) =>
-      same_skel_tm σ t11 t21 ∧ same_skel_tm σ t12 t22
+      same_skel_tm t11 t21 ∧ same_skel_tm t12 t22
     | (tproj t1 l1, tproj t2 l2) =>
-      same_skel_tm σ t1 t2 ∧ l1 = l2
+      same_skel_tm t1 t2 ∧ l1 = l2
     | _ => False
     end
   with
-  same_skel_vl (σ: vls) (v1 v2: vl): Prop :=
+  same_skel_vl (v1 v2: vl): Prop :=
     match (v1, v2) with
     | (var_vl i1, var_vl i2) => i1 = i2
-    | (vabs t1, vabs t2) => same_skel_tm (push_var σ) t1 t2
-    | (vobj ds1, vobj ds2) => same_skel_dms (push_var σ) ds1 ds2
+    | (vabs t1, vabs t2) => same_skel_tm t1 t2
+    | (vobj ds1, vobj ds2) => same_skel_dms ds1 ds2
     | _ => False
     end
   with
-  same_skel_dms (σ: vls) (ds1 ds2: dms): Prop :=
+  same_skel_dms (ds1 ds2: dms): Prop :=
     match (ds1, ds2) with
     | (dnil, dnil) => True
     | (dcons d1 ds1, dcons d2 ds2) =>
-      same_skel_dm σ d1 d2 ∧ same_skel_dms σ ds1 ds2
+      same_skel_dm d1 d2 ∧ same_skel_dms ds1 ds2
     | _ => False
     end
   with
-  same_skel_dm (σ: vls) (d1 d2: dm): Prop :=
+  same_skel_dm (d1 d2: dm): Prop :=
     match (d1, d2) with
     | (dtysyn T1, dtysem σ2 γ2) =>
       (* Only nontrivial case *)
       True
-    | (dvl v1, dvl v2) => same_skel_vl σ v1 v2
+    | (dvl v1, dvl v2) => same_skel_vl v1 v2
     | _ => False
     end
   with
-  same_skel_path (σ: vls) (p1 p2: path): Prop :=
+  same_skel_path (p1 p2: path): Prop :=
     match (p1, p2) with
-    | (pv v1, pv v2) => same_skel_vl σ v1 v2
-    | (pself p1 l1, pself p2 l2) => same_skel_path σ p1 p2 ∧ l1 = l2
+    | (pv v1, pv v2) => same_skel_vl v1 v2
+    | (pself p1 l1, pself p2 l2) => same_skel_path p1 p2 ∧ l1 = l2
     | _ => False
     end
   with
-  same_skel_ty (σ: vls) (T1 T2: ty): Prop :=
+  same_skel_ty (T1 T2: ty): Prop :=
     match (T1, T2) with
     | (TTop, TTop) => True
     | (TBot, TBot) => True
     | (TAnd T11 T12, TAnd T21 T22) =>
-      same_skel_ty σ T11 T21 ∧ same_skel_ty σ T12 T22
+      same_skel_ty T11 T21 ∧ same_skel_ty T12 T22
     | (TOr T11 T12, TOr T21 T22) =>
-      same_skel_ty σ T11 T21 ∧ same_skel_ty σ T12 T22
+      same_skel_ty T11 T21 ∧ same_skel_ty T12 T22
     | (TLater T1, TLater T2) =>
-      same_skel_ty σ T1 T2
+      same_skel_ty T1 T2
     | (TAll T11 T12, TAll T21 T22) =>
-      same_skel_ty σ T11 T21 ∧ same_skel_ty (push_var σ) T12 T22
+      same_skel_ty T11 T21 ∧ same_skel_ty T12 T22
     | (TMu T1, TMu T2) =>
-      same_skel_ty (push_var σ) T1 T2
-    | (TVMem l1 T1, TVMem l2 T2) => l1 = l2 ∧ same_skel_ty σ T1 T2
-    | (TTMem l1 T11 T12, TTMem l2 T21 T22) => l1 = l2 ∧ same_skel_ty σ T11 T21 ∧ same_skel_ty σ T12 T22
-    | (TSel p1 l1, TSel p2 l2) => same_skel_path σ p1 p2 ∧ l1 = l2
-    | (TSelA p1 l1 T11 T12, TSelA p2 l2 T21 T22) => same_skel_path σ p1 p2 ∧ l1 = l2 ∧ same_skel_ty σ T11 T21 ∧ same_skel_ty σ T12 T22
+      same_skel_ty T1 T2
+    | (TVMem l1 T1, TVMem l2 T2) => l1 = l2 ∧ same_skel_ty T1 T2
+    | (TTMem l1 T11 T12, TTMem l2 T21 T22) => l1 = l2 ∧ same_skel_ty T11 T21 ∧ same_skel_ty T12 T22
+    | (TSel p1 l1, TSel p2 l2) => same_skel_path p1 p2 ∧ l1 = l2
+    | (TSelA p1 l1 T11 T12, TSelA p2 l2 T21 T22) => same_skel_path p1 p2 ∧ l1 = l2 ∧ same_skel_ty T11 T21 ∧ same_skel_ty T12 T22
     | _ => False
     end.
 
   Lemma translation_same_skel σ t t':
-    ( t_tm σ t t' → ⌜same_skel_tm σ t t'⌝)%I
+    ( t_tm σ t t' → ⌜same_skel_tm t t'⌝)%I
   with translation_same_ty σ t t':
-    ( t_ty σ t t' → ⌜same_skel_ty σ t t'⌝)%I
+    ( t_ty σ t t' → ⌜same_skel_ty t t'⌝)%I
   with translation_same_path σ t t':
-    ( t_path σ t t' → ⌜same_skel_path σ t t'⌝)%I
+    ( t_path σ t t' → ⌜same_skel_path t t'⌝)%I
   with translation_same_dm σ t t':
-    ( t_dm σ t t' → ⌜same_skel_dm σ t t'⌝)%I
+    ( t_dm σ t t' → ⌜same_skel_dm t t'⌝)%I
   with translation_same_skel_dms σ t t':
-    ( t_dms σ t t' → ⌜same_skel_dms σ t t'⌝)%I
+    ( t_dms σ t t' → ⌜same_skel_dms t t'⌝)%I
   with translation_same_skel_vl σ t t':
-    ( t_vl σ t t' → ⌜same_skel_vl σ t t'⌝)%I.
+    ( t_vl σ t t' → ⌜same_skel_vl t t'⌝)%I.
   Proof.
     all: iIntros "Hyp";
       destruct t; destruct t'; simpl; eauto;
@@ -345,4 +347,68 @@ Section Sec.
       end.
   Qed.
 
+  Fixpoint same_skel_ectx K K' :=
+    match K, K' with
+    | AppLCtx e2, AppLCtx e2' => same_skel_tm e2 e2'
+    | AppRCtx v1, AppRCtx v1' => same_skel_vl v1 v1'
+    | ProjCtx l, ProjCtx l' => l = l'
+    | _, _ => False
+    end.
+
+  Definition same_skel_list_ectx Ks Ks' :=
+    List.Forall2 same_skel_ectx Ks Ks'.
+
+  Lemma same_skel_fill Ks e t':
+    same_skel_tm (fill Ks e) t' →
+    exists Ks' e',  t' = fill Ks' e' ∧ same_skel_tm e e' ∧ same_skel_list_ectx Ks Ks'.
+  Proof. Admitted.
+
+  Lemma same_skel_fill_item Ks Ks' e e':
+    same_skel_list_ectx Ks Ks' →
+    same_skel_tm e e' →
+    same_skel_tm (fill Ks e) (fill Ks' e').
+  Admitted.
+
+
+  Lemma same_skel_subst e e' v v':
+    same_skel_tm e e' → same_skel_vl v v' →
+    same_skel_tm (e.[v/]) (e'.[v'/]).
+  Proof.
+  Admitted.
+
+  Lemma same_skel_dms_index ds ds' v l:
+    same_skel_dms ds ds' →
+    index_dms l (selfSubst ds) = Some (dvl v) →
+    exists v', index_dms l (selfSubst ds') = Some (dvl v') ∧ same_skel_vl v v'.
+  Proof.
+  Admitted.
+
+  Ltac destruct_matches :=
+    repeat progress match goal with
+                    | H: match ?t with | _ => _ end |- _ => destruct t; try done
+                    | H: ?A ∧ ?B |- _ => destruct H
+                    end.
+
+   Lemma simulation_skeleton_head t1' t1 t2 σ σ' ts:
+    same_skel_tm t1 t1' →
+    head_step t1 σ [] t2 σ' ts →
+    exists t2', head_step t1' σ [] t2' σ' ts ∧ same_skel_tm t2 t2'.
+  Proof.
+    move=> Hsk Hhs. inversion Hhs; subst; simpl in *.
+    - destruct_matches. eexists. split; first by econstructor. by eapply same_skel_subst.
+    - destruct_matches. subst. destruct (same_skel_dms_index ds d v l0 H1 H0) as [? [? ?]]. eexists.
+      split; [by econstructor | done].
+  Qed.
+
+  Theorem simulation_skeleton t1 t1' t2 σ σ' ts:
+    same_skel_tm t1 t1' →
+    prim_step t1 σ [] t2 σ' ts →
+    exists t2', prim_step t1' σ [] t2' σ' ts ∧ same_skel_tm t2 t2'.
+  Proof.
+    move=> Hsk Hstep. rewrite /prim_step in Hstep. simpl in *.
+    inversion Hstep; subst; simpl in *.
+    apply same_skel_fill in Hsk as [Ks' [e' [Hfill [Hskel Hsklsit]]]].  simpl in *.
+    eapply simulation_skeleton_head in H2 as [e'' [Hhs Hskk]]; last by eauto.
+    exists (fill Ks' e''). subst. split; [econstructor; eauto | by apply same_skel_fill_item].
+  Qed.
 End Sec.
